define the protocol and prove the constructor

theories/logatom_stack/stack.v
@@ -1,28 +1,37 @@
-From iris.algebra Require Import excl.
+From iris.heap_lang Require Export lifting notation.
+From iris.algebra Require Import excl auth list.
 From iris.base_logic.lib Require Import invariants.
 From iris.program_logic Require Import atomic.
 From iris.proofmode Require Import tactics.
-From iris.heap_lang Require Import lifting proofmode notation atomic_heap par.
+From iris.heap_lang Require Import proofmode notation atomic_heap par.
 From iris.bi.lib Require Import fractional.
 Set Default Proof Using "Type".
 
 (** * Implement a concurrent stack with helping on top of an arbitrary atomic
 heap. *)
+Definition stackN : namespace := nroot .@ "logatom_stack".
+Definition offerN : namespace := nroot .@ "logatom_stack" .@ "offer".
+Definition protoN : namespace := nroot .@ "logatom_stack" .@ "protocol".
 
 (** The CMRA & functor we need. *)
 (* Not bundling heapG, as it may be shared with other users. *)
-Class stackG Σ := StackG { stack_tokG :> inG Σ (exclR unitC) }.
-Definition stackΣ : gFunctors := #[GFunctor (exclR unitC)].
+Class stackG Σ := StackG {
+  stack_tokG :> inG Σ (exclR unitC);
+  stack_stateG :> inG Σ (authR (optionUR $ exclR (listC valC)));
+ }.
+Definition stackΣ : gFunctors :=
+  #[GFunctor (exclR unitC); GFunctor (authR (optionUR $ exclR (listC valC)))].
 
 Instance subG_stackΣ {Σ} : subG stackΣ Σ → stackG Σ.
 Proof. solve_inG. Qed.
 
 Section stack.
   Context `{!heapG Σ, stackG Σ} {aheap: atomic_heap Σ}.
+  Notation iProp := (iProp Σ).
 
   Import atomic_heap.notation.
 
-  (** Code. A stack is a pair of two option pointers-to-pointers, one for the
+  (** Code. A stack is a pair of two pointers-to-option-pointers, one for the
   head element (if the stack is non-empty) and for the current offer (if it
   exists).  A stack element is a pair of a value an an optional pointer to the
   next element. *)
@@ -80,4 +89,74 @@ Section stack.
           end
       end.
 
+  (** Invariant and protocol. *)
+  Definition stack_content (γs : gname) (l : list val) : iProp :=
+    (own γs (◯ Excl' l))%I.
+  Global Instance stack_content_timeless γs l : Timeless (stack_content γs l) := _.
+
+  Fixpoint list_inv (l : list val) (rep : val) : iProp :=
+    match l with
+    | nil => ⌜rep = NONEV⌝
+    | v::l => ∃ (ℓ : loc) (rep' : val), ⌜rep = SOMEV #ℓ⌝ ∗ ℓ ↦ (v, rep') ∗ list_inv l rep'
+    end%I.
+
+  Inductive offer_state := OfferPending | OfferRevoked | OfferAccepted | OfferAcked.
+
+  Definition offer_state_rep (st : offer_state) : Z :=
+    match st with
+    | OfferPending => 0
+    | OfferRevoked => 2
+    | OfferAccepted => 1
+    | OfferAcked => 1
+    end.
+
+  Definition offer_inv (st_loc : loc) (γo : gname) (P Q : iProp) : iProp :=
+    (∃ st : offer_state, st_loc ↦ #(offer_state_rep st) ∗
+      match st with
+      | OfferPending => P
+      | OfferAccepted => Q
+      | _ => True
+      end)%I.
+
+  Definition is_offer (γs : gname) (offer_rep : option (val * loc)) :=
+    match offer_rep with
+    | None => True
+    | Some (v, st_loc) =>
+      ∃ P Q γo, inv offerN (offer_inv st_loc γo P Q) ∗
+                (* The persistent part of the Laterable AU *)
+                □ (▷ P -∗ ◇ AU << ∀ l, stack_content γs l >> @ ⊤∖↑stackN, ∅
+                               << stack_content γs (v::l), COMM Q >>)
+    end%I.
+
+  Definition offer_to_val (offer_rep : option (val * loc)) : val :=
+    match offer_rep with
+    | None => NONEV
+    | Some (v, l) => SOMEV (v, #l)
+    end.
+
+  Definition stack_inv (γs : gname) (head : loc) (offer : loc) : iProp :=
+    (∃ stack_rep offer_rep l, own γs (● Excl' l) ∗
+       head ↦ stack_rep ∗ list_inv l stack_rep ∗
+       offer ↦ offer_to_val offer_rep ∗ is_offer γs offer_rep)%I.
+
+  Definition is_stack (γs : gname) (s : val) : iProp :=
+    (∃ head offer : loc, ⌜s = (#head, #offer)%V⌝ ∗ inv protoN (stack_inv γs head offer))%I.
+  Global Instance is_stack_persistent γs s : Persistent (is_stack γs s) := _.
+
+  (** Proofs. *)
+  Lemma new_stack_spec :
+    {{{ True }}} new_stack #() {{{ γs s, RET s; is_stack γs s ∗ stack_content γs [] }}}.
+  Proof.
+    iIntros (Φ) "_ HΦ". iApply wp_fupd. wp_lam.
+    wp_apply alloc_spec; first done. iIntros (head) "Hhead". wp_let.
+    wp_apply alloc_spec; first done. iIntros (offer) "Hoffer". wp_let.
+    iMod (own_alloc (● Excl' [] ⋅ ◯ Excl' [])) as (γs) "[Hs● Hs◯]".
+    { apply auth_valid_discrete_2. split; done. }
+    iMod (inv_alloc protoN _ (stack_inv γs head offer) with "[-HΦ Hs◯]").
+    { iNext. iExists _, None, _. iFrame. done. }
+    iApply "HΦ". iFrame "Hs◯". iModIntro. iExists _, _. auto.
+  Qed.
+
 End stack.
+
+Global Typeclasses Opaque stack_content is_stack.
